src/typechecker/FStar.TypeChecker.Common.fsti
@@ -13,7 +13,6 @@
    See the License for the specific language governing permissions and
    limitations under the License.
 *)
-#light "off"
 module FStar.TypeChecker.Common
 open Prims
 open FStar.Pervasives
@@ -43,26 +42,26 @@ type rank_t =
     | Rigid_flex
     | Flex_flex
 
-type problem<'a> = {                  //Try to prove: lhs rel rhs ~> guard
+type problem 'a = {                  //Try to prove: lhs rel rhs ~ guard
     pid:int;
     lhs:'a;
     relation:rel;
     rhs:'a;
-    element:option<bv>;               //where, guard is a predicate on this term (which appears free in/is a subterm of the guard)
+    element:option bv;               //where, guard is a predicate on this term (which appears free in/is a subterm of the guard)
     logical_guard:term;               //the condition under which this problem is solveable; (?u v1..vn)
     logical_guard_uvar:ctx_uvar;
-    reason: list<string>;             //why we generated this problem, for error reporting
+    reason: list string;             //why we generated this problem, for error reporting
     loc: Range.range;                 //and the source location where this arose
-    rank: option<rank_t>;
+    rank: option rank_t;
 }
 
 type prob =
-  | TProb of problem<typ>
-  | CProb of problem<comp>
+  | TProb of problem typ
+  | CProb of problem comp
 
-val as_tprob : prob -> problem<typ>
+val as_tprob : prob -> problem typ
 
-type probs = list<prob>
+type probs = list prob
 
 type guard_formula =
   | Trivial
@@ -81,14 +80,14 @@ type deferred_reason =
   | Deferred_delay_match_heuristic
   | Deferred_to_user_tac
 
-type deferred = list<(deferred_reason * string * prob)>
+type deferred = list (deferred_reason * string * prob)
 
 type univ_ineq = universe * universe
 
 val mk_by_tactic : term -> term -> term
 
 val delta_depth_greater_than : delta_depth -> delta_depth -> bool
-val decr_delta_depth : delta_depth -> option<delta_depth>
+val decr_delta_depth : delta_depth -> option delta_depth
 
 (***********************************************************************************)
 (* A table of file -> starting row -> starting col -> identifier info              *)
@@ -101,27 +100,27 @@ val decr_delta_depth : delta_depth -> option<delta_depth>
 (***********************************************************************************)
 
 type identifier_info = {
-    identifier:either<bv, fv>;
+    identifier:either bv fv;
     identifier_ty:typ;
     identifier_range:Range.range;
 }
 
-val insert_col_info : int -> identifier_info -> list<(int * identifier_info)> -> list<(int * identifier_info)>
-val find_nearest_preceding_col_info : int -> list<(int * identifier_info)> -> option<identifier_info>
+val insert_col_info : int -> identifier_info -> list (int * identifier_info) -> list (int * identifier_info)
+val find_nearest_preceding_col_info : int -> list (int * identifier_info) -> option identifier_info
 
 type id_info_by_col = //sorted in ascending order of columns
-    list<(int * identifier_info)>
+    list (int * identifier_info)
 
 type col_info_by_row =
-    BU.pimap<id_info_by_col>
+    BU.pimap id_info_by_col
 
 type row_info_by_file =
-    BU.psmap<col_info_by_row>
+    BU.psmap col_info_by_row
 
 type id_info_table = {
     id_info_enabled: bool;
     id_info_db: row_info_by_file;
-    id_info_buffer: list<identifier_info>;
+    id_info_buffer: list identifier_info;
 }
 val id_info_table_empty : id_info_table
 
@@ -129,7 +128,7 @@ val id_info_insert_bv : id_info_table -> bv -> typ -> id_info_table
 val id_info_insert_fv : id_info_table -> fv -> typ -> id_info_table
 val id_info_toggle    : id_info_table -> bool -> id_info_table
 val id_info_promote   : id_info_table -> (typ -> typ) -> id_info_table
-val id_info_at_pos    : id_info_table -> string -> int -> int -> option<identifier_info>
+val id_info_at_pos    : id_info_table -> string -> int -> int -> option identifier_info
 
 // Reason, term and uvar, and (rough) position where it is introduced
 // The term is just a Tm_uvar of the ctx_uvar
@@ -139,7 +138,7 @@ type implicit = {
     imp_tm     : term;                    // The term, made up of the ctx_uvar
     imp_range  : Range.range;             // Position where it was introduced
 }
-type implicits = list<implicit>
+type implicits = list implicit
 
 val implicits_to_string : implicits -> string
 
@@ -148,7 +147,7 @@ type guard_t = {
   deferred_to_tac: deferred; //This field maintains problems that are to be dispatched to a tactic
                              //They are never attempted by the unification engine in Rel
   deferred:   deferred;
-  univ_ineqs: list<universe> * list<univ_ineq>;
+  univ_ineqs: list universe * list univ_ineq;
   implicits:  implicits;
 }
 
@@ -157,26 +156,26 @@ val trivial_guard : guard_t
 val conj_guard    : guard_t -> guard_t -> guard_t
 val check_trivial : term -> guard_formula
 val imp_guard     : guard_t -> guard_t -> guard_t
-val conj_guards   : list<guard_t> -> guard_t
+val conj_guards   : list guard_t -> guard_t
 
 val weaken_guard_formula: guard_t -> typ -> guard_t
 type lcomp = { //a lazy computation
     eff_name: lident;
     res_typ: typ;
-    cflags: list<cflag>;
-    comp_thunk: ref<(either<(unit -> (comp * guard_t)), comp>)>
+    cflags: list cflag;
+    comp_thunk: ref (either (unit -> (comp * guard_t)) comp)
 }
 
 val mk_lcomp:
     eff_name: lident ->
     res_typ: typ ->
-    cflags: list<cflag> ->
+    cflags: list cflag ->
     comp_thunk: (unit -> (comp * guard_t)) -> lcomp
 
 val lcomp_comp: lcomp -> (comp * guard_t)
 val apply_lcomp : (comp -> comp) -> (guard_t -> guard_t) -> lcomp -> lcomp
 val lcomp_to_string : lcomp -> string
-val lcomp_set_flags : lcomp -> list<S.cflag> -> lcomp
+val lcomp_set_flags : lcomp -> list S.cflag -> lcomp
 val is_total_lcomp : lcomp -> bool
 val is_tot_or_gtot_lcomp : lcomp -> bool
 val is_lcomp_partial_return : lcomp -> bool
