src/typechecker/FStar.TypeChecker.NBE.fsti
@@ -15,7 +15,6 @@
    See the License for the specific language governing permissions and
    limitations under the License.
 *)
-#light "off"
 module FStar.TypeChecker.NBE
 open FStar.Pervasives
 open FStar.Compiler.Effect
@@ -30,13 +29,13 @@ open FStar.TypeChecker.Normalize
 open FStar.TypeChecker.NBETerm
 module Cfg = FStar.TypeChecker.Cfg
 
-val normalize_for_unit_test : steps:list<Env.step>
+val normalize_for_unit_test : steps:list Env.step
                -> env : Env.env
                -> e:term
                -> term
 
-val normalize   : list<Cfg.primitive_step>
-                -> list<Env.step>
+val normalize   : list Cfg.primitive_step
+                -> list Env.step
                 -> Env.env
                 -> term
                 -> term
