src/typechecker/FStar.TypeChecker.Rel.fsti
@@ -13,7 +13,7 @@
    See the License for the specific language governing permissions and
    limitations under the License.
 *)
-#light "off"
+
 module FStar.TypeChecker.Rel
 open FStar.Pervasives
 open FStar.Compiler.Effect
@@ -39,7 +39,7 @@ val flex_prob_closing         : env -> binders -> prob -> bool
 //val is_trivial_guard_formula  : guard_t -> bool
 //val conj_guard                : guard_t -> guard_t -> guard_t
 //val abstract_guard            : binder -> guard_t -> guard_t
-//val abstract_guard_n          : list<binder> -> guard_t -> guard_t
+//val abstract_guard_n          : list binder> -> guard_t - guard_t
 //val imp_guard                 : guard_t -> guard_t -> guard_t
 //val guard_of_guard_formula    : guard_formula -> guard_t
 //val guard_form                : guard_t -> guard_formula
@@ -52,23 +52,23 @@ val discharge_guard           : env -> guard_t -> guard_t
 val force_trivial_guard       : env -> guard_t -> unit
 val resolve_implicits         : env -> guard_t -> guard_t
 val resolve_implicits_tac     : env -> guard_t -> guard_t
-val base_and_refinement_maybe_delta : bool -> env -> term -> term * option<(bv * term)>
-val base_and_refinement       : env -> term -> term * option<(bv * term)>
+val base_and_refinement_maybe_delta : bool -> env -> term -> term * option (bv * term)
+val base_and_refinement       : env -> term -> term * option (bv * term)
 
 val unrefine   : env -> typ -> typ
-val try_teq    : bool -> env -> typ -> typ -> option<guard_t>
+val try_teq    : bool -> env -> typ -> typ -> option guard_t
 val teq        : env -> typ -> typ -> guard_t
-val get_teq_predicate : env -> typ -> typ -> option<guard_t>
+val get_teq_predicate : env -> typ -> typ -> option guard_t
 val teq_force  : env -> typ -> typ -> unit
-val teq_nosmt        : env -> typ -> typ -> option<guard_t>
+val teq_nosmt        : env -> typ -> typ -> option guard_t
 val teq_nosmt_force  : env -> typ -> typ -> bool
-val layered_effect_teq : env -> typ -> typ -> reason:option<string> -> guard_t
-val get_subtyping_predicate: env -> typ -> typ -> option<guard_t>
-val get_subtyping_prop: env -> typ -> typ -> option<guard_t>
-val subtype_nosmt       : env -> typ -> typ -> option<guard_t>
+val layered_effect_teq : env -> typ -> typ -> reason:option string -> guard_t
+val get_subtyping_predicate: env -> typ -> typ -> option guard_t
+val get_subtyping_prop: env -> typ -> typ -> option guard_t
+val subtype_nosmt       : env -> typ -> typ -> option guard_t
 val subtype_nosmt_force : env -> typ -> typ -> bool
-val sub_comp   : env -> comp -> comp -> option<guard_t>
-val eq_comp : env -> comp -> comp -> option<guard_t>
+val sub_comp   : env -> comp -> comp -> option guard_t
+val eq_comp : env -> comp -> comp -> option guard_t
 
 val universe_inequality : universe -> universe -> guard_t
 
